ChronoFold.lean
@@ -1,3 +1,0 @@
-def hello : String := "ChronoFold Alive"
-
-#eval hello
